#+TITLE: 2024.1 How is $a^* = 1/(1-a)?$
#+AUTHOR: Benjamin Lucien Kaminski
#+EMAIL: kaminski@cs.uni-saarland.de
#+DATE: <2024-06-21>
#+LAYOUT: post
#+TAGS: Kleene algebra

Consider the language \(a^*\).
We have
\begin{align*}
		a^* &{}= \varepsilon + a + aa + aaa + \ldots\\
		&{}= 1 + a + a^2 + a^3 + \ldots~, \tag{since \(\varepsilon\) is the unit of concatenation}\\
		&{}= \sum_{k = 0}^\infty a^k
\end{align*}
in which we now immediately recognize the familiar \emph{geometric series} whose closed form is well known to be \(\frac{1}{1 - a}\).
In that sense,
\begin{align*}
		a^* = \frac{1}{1 - a}~.
\end{align*}

{{{teaser_end}}}

We have to be a bit careful as the above is actually a non-commutative division (since multiplication of words is non-commutative), so we write
{{{raw}}}
\begin{align*}
	\frac{{|}\,a~}{~b\,{|}}
 	\quad\text{for}\quad
	\frac{1}{b} \cdot a
	\qquad\text{and}\qquad
	\frac{~a\,{|}}{{|}\,b~}
	\quad\text{for}\quad{}
	a \cdot \frac{1}{b}~,
\end{align*}
whereas \(\frac{{|}\,1~}{~b\,{|}} = \frac{~1\,{|}}{{|}\,b~} = \frac{1}{b}\) because \(\varepsilon \cdot x = x \cdot \varepsilon = x\).
{{{endraw}}}

Using our new insight  -- "Kleene star is a fraction" --, we can now conveniently prove, for instance, the well-known identity \(a(ba)^* = (ab)^*a\). 
While the standard proof is rather lengthy and involves several axioms of Kleene algebra, our proof fits on a beer coaster (it was actually devised on such, see picture below) and goes as follows:
{{{raw}}}
\begin{align*}
	a(ba)^* 
	&{} = \frac{\quad{}~a~\quad{|}}{{|}\,1 - ba}\\
	&{} = \frac{\quad{}1\quad{|}}{{|}\,\frac{1}{a} - b}
	\tag{right-expand fraction by \(\frac{1}{a}\)}\\
	&{} = \frac{{|}\quad{}~1~\quad}{\frac{1}{a} - b\,{|}}
	\tag{by \(\frac{{|}\,1~}{~x\,{|}} = \frac{~1\,{|}}{{|}\,x~}\)}\\
	&{} = \frac{{|}\quad{}~a~\quad}{1 - ab\,{|}}
	\tag{left-expand fraction by \(a\)}\\
	 &{} =(ab)^*a
\end{align*}
{{{endraw}}}
There are "only" two problems with all of the above: neither \({\ldots} - a\) nor \(\tfrac{1}{\ldots}\) make sense at the moment.

Open Problem: How can we formally make sense of additive and multiplicative inverses on words, such that \(a^* = 1 + a + a^2 + {\dots} = \frac{1}{1 - a}\), i.e.\ such that \(a^* \cdot (1 - a) = 1\)?
